Got rid of one_shot

tests/joining_existentials.v
@@ -1,8 +1,17 @@
-From iris.program_logic Require Import saved_one_shot hoare.
+From iris.algebra Require Import csum.
+From iris.program_logic Require Import hoare.
 From iris.heap_lang.lib.barrier Require Import proof specification.
 From iris.heap_lang Require Import notation par proofmode.
 From iris.proofmode Require Import invariants.
 Import uPred.
+
+Class oneShotG (Λ : language) (Σ : gFunctors) (F : cFunctor) :=
+  one_shot_inG :>
+    inG Λ Σ (csumR (exclR unitC) (agreeR $ laterC $ F (iPrePropG Λ Σ))).
+Definition oneShotGF (F : cFunctor) : gFunctor :=
+  GFunctor (csumRF (exclRF unitC) (agreeRF (▶ F))).
+Instance inGF_oneShotG  `{inGF Λ Σ (oneShotGF F)} : oneShotG Λ Σ F.
+Proof. apply: inGF_inG. Qed.
 
 Definition client eM eW1 eW2 : expr [] :=
   let: "b" := newbarrier #() in
@@ -17,7 +26,8 @@ Local Notation iProp := (iPropG heap_lang Σ).
 Local Notation X := (G iProp).
 
 Definition barrier_res γ (Φ : X → iProp) : iProp :=
-  (∃ x, one_shot_own γ x ★ Φ x)%I.
+  (∃ x, own γ (Cinr $ to_agree $
+               Next (cFunctor_map G (iProp_fold, iProp_unfold) x)) ★ Φ x)%I.
 
 Lemma worker_spec e γ l (Φ Ψ : X → iProp) :
   recv heapN N l (barrier_res γ Φ) ★ (∀ x, {{ Φ x }} e {{ _, Ψ x }})
@@ -43,7 +53,13 @@ Lemma Q_res_join γ : barrier_res γ Ψ1 ★ barrier_res γ Ψ2 ⊢ ▷ barrier_
 Proof.
   iIntros "[Hγ Hγ']";
   iDestruct "Hγ" as {x} "[#Hγ Hx]"; iDestruct "Hγ'" as {x'} "[#Hγ' Hx']".
-  iDestruct (one_shot_agree γ x x' with "[#]") as "Hxx"; first (by iSplit).
+  iAssert (▷ (x ≡ x'):iProp)%I as "Hxx" .
+  { iCombine "Hγ" "Hγ'" as "Hγ2". iClear "Hγ Hγ'".
+    rewrite own_valid csum_validI /= agree_validI agree_equivI later_equivI /=.
+    rewrite -{2}[x]cFunctor_id -{2}[x']cFunctor_id.
+    rewrite (ne_proper (cFunctor_map G) (cid, cid) (_ ◎ _, _ ◎ _)).
+    2:by split; intro; simpl; symmetry; apply iProp_fold_unfold.
+    rewrite !cFunctor_compose. iNext. by iRewrite "Hγ2". }
   iNext. iRewrite -"Hxx" in "Hx'".
   iExists x; iFrame "Hγ". iApply Ψ_join; by iSplitL "Hx".
 Qed.
@@ -57,7 +73,7 @@ Lemma client_spec_new (eM eW1 eW2 : expr []) (eM' eW1' eW2' : expr ("b" :b: []))
   ⊢ WP client eM' eW1' eW2' {{ _, ∃ γ, barrier_res γ Ψ }}.
 Proof.
   iIntros {HN -> -> ->} "/= (#Hh&HP&#He&#He1&#He2)"; rewrite /client.
-  iPvs one_shot_alloc as {γ} "Hγ".
+  iPvs (own_alloc (Cinl (Excl ()))) as {γ} "Hγ". done.
   wp_apply (newbarrier_spec heapN N (barrier_res γ Φ)); auto.
   iFrame "Hh". iIntros {l} "[Hr Hs]".
   set (workers_post (v : val) := (barrier_res γ Ψ1 ★ barrier_res γ Ψ2)%I).
@@ -65,7 +81,8 @@ Proof.
   iFrame "Hh". iSplitL "HP Hs Hγ"; [|iSplitL "Hr"].
   - wp_focus eM. iApply wp_wand_l; iSplitR "HP"; [|by iApply "He"].
     iIntros {v} "HP"; iDestruct "HP" as {x} "HP". wp_let.
-    iPvs (one_shot_init _ _ x with "Hγ") as "Hx".
+    iPvs (own_update _ _ (Cinr (to_agree _)) with "Hγ") as "Hx".
+    by apply cmra_update_exclusive.
     iApply signal_spec; iFrame "Hs"; iSplit; last done.
     iExists x; auto.
   - iDestruct (recv_weaken with "[] Hr") as "Hr"; first by iApply P_res_split.
